Start thinking about how to stitch everything together to prove we actually did HMAC.  Checkpointing before pulling bswap out everywhere.

verified/sha/memory-helpers.i.dfy
@@ -15,7 +15,6 @@ lemma lemma_ValidMemRange_offset(base:int, count:nat)
     //assert ValidMem(limit);
 }
 
-
 function AddrMemContentsSeq(m:memmap, begin_ptr:nat, count:nat) : seq<word>
   requires ValidAddrMemStateOpaque(m);
   requires count > 0 ==> ValidMemRange(begin_ptr, begin_ptr + count * WORDSIZE);
@@ -27,6 +26,21 @@ function AddrMemContentsSeq(m:memmap, begin_ptr:nat, count:nat) : seq<word>
   else
       lemma_ValidMemRange_offset(begin_ptr, count);
       [AddrMemContents(m, begin_ptr)] + AddrMemContentsSeq(m, begin_ptr + WORDSIZE, count - 1)
+}
+
+lemma lemma_AddrMemContentsSeq_adds(m:memmap, begin_ptr:nat, count:nat, count':nat)
+  requires ValidAddrMemStateOpaque(m);
+  requires count > 0 ==> ValidMemRange(begin_ptr, begin_ptr + count * WORDSIZE);
+  requires count' < count;
+  decreases count;
+  ensures  count - count' > 0 ==> ValidMemRange(begin_ptr + count' * WORDSIZE, begin_ptr + (count - count') * WORDSIZE);
+  ensures  AddrMemContentsSeq(m, begin_ptr, count) == AddrMemContentsSeq(m, begin_ptr, count') 
+                                                    + AddrMemContentsSeq(m, begin_ptr + count' * WORDSIZE, count - count') 
+{
+    if count' == 0 {
+    } else {
+        lemma_AddrMemContentsSeq_adds(m, begin_ptr + WORDSIZE, count - 1, count' - 1);
+    }
 }
 
 lemma lemma_AddrMemContentsSeq_framing(m:memmap, m':memmap, begin_ptr:nat, count:nat, l1:nat, h1:nat, l2:nat, h2:nat)
@@ -41,6 +55,7 @@ lemma lemma_AddrMemContentsSeq_framing(m:memmap, m':memmap, begin_ptr:nat, count
 {
     if count == 0 {
     } else {
+        lemma_ValidMemRange_offset(begin_ptr, count);
         lemma_AddrMemContentsSeq_framing(m, m', begin_ptr + WORDSIZE, count - 1, l1, h1, l2, h2);
     }
 }
