verified/sha/hmac-helpers.i.dfy
@@ -1,0 +1,34 @@
+include "memory-helpers.i.dfy"
+
+lemma lemma_apply_opad_complete(m:memmap, m':memmap, base:nat, count:nat)
+    requires ValidAddrMemStateOpaque(m) && ValidAddrMemStateOpaque(m');
+    requires count > 0 ==> ValidMemRange(base, base + count * WORDSIZE);
+    requires forall a :: base <= a < base + count * WORDSIZE && WordAligned(a) 
+                     ==> AddrMemContents(m', a) == BitwiseXor(AddrMemContents(m, a), 0x5c5c5c5c); 
+    ensures  AddrMemContentsSeq(m', base, count) == 
+      SeqXor(AddrMemContentsSeq(m, base, count), Opad(count));
+
+{
+  if count == 0 {
+	} else {
+		lemma_ValidMemRange_offset(base, count);
+		lemma_apply_opad_complete(m, m', base, count - 1);
+	}
+}
+
+
+lemma lemma_apply_ipad_complete(m:memmap, m':memmap, base:nat, count:nat)
+    requires ValidAddrMemStateOpaque(m) && ValidAddrMemStateOpaque(m');
+    requires count > 0 ==> ValidMemRange(base, base + count * WORDSIZE);
+    requires forall a :: base <= a < base + count * WORDSIZE && WordAligned(a) 
+                     ==> AddrMemContents(m', a) == BitwiseXor(AddrMemContents(m, a), 0x36363636); 
+    ensures  AddrMemContentsSeq(m', base, count) == 
+      SeqXor(AddrMemContentsSeq(m, base, count), Ipad(count));
+
+{
+  if count == 0 {
+	} else {
+		lemma_ValidMemRange_offset(base, count);
+		lemma_apply_ipad_complete(m, m', base, count - 1);
+	}
+}
